Fir/Wasm/Concrete/ReferenceCountCorrectness.lean
@@ -721,6 +721,7 @@ theorem ConstructorObjectRel.writeReferenceCount
     semanticUSizeFields := related.semanticUSizeFields
     semanticScalarFields := scalarFieldsAfter
     fieldKindsSize := related.fieldKindsSize
+    fieldKindsValid := related.fieldKindsValid
     objectFields := ?_
     usizeFields := ?_ }
   · intro index kind value kindAt valueAt
